feat(eq): prove canonical bind congruence

theories/Eq/ProbabilisticEutt.v
@@ -3,6 +3,7 @@ Set Warnings "-ambiguous-paths".
 Set Universe Polymorphism.
 
 Require Import Program.
+From Coq Require Import Logic.ClassicalChoice.
 From Coinduction Require Import all.
 From mathcomp Require Import ssreflect.
 From PTree.Core Require Import PTreeDefinitionNew.
@@ -615,3 +616,204 @@ Proof.
 Qed.
 
 End ProbabilisticEuttStructuralLaws.
+
+Section ProbabilisticEuttBindCongruence.
+Context {E : Type -> Type} {MN MF : Type -> Type}
+  `{NI : SemanticMeasureInterface MN}
+  `{FI : SemanticMeasureInterface MF}
+  `{NC : @SemanticMeasureCoreLaws MN NI}
+  `{FC : @SemanticMeasureCoreLaws MF FI}
+  `{FB : @SemanticMeasureBindLaws MF FI}
+  `{MX : MixedMeasureInterface MN MF}
+  `{ML : @MixedMeasureLaws MN MF NI FI MX}
+  `{FO : @SemanticOmegaInterface MF FI}
+  `{FOrd : @SemanticMeasureOrderLaws MF FI FO}
+  `{FOL : @SemanticOmegaLaws MF FI FO}
+  `{FCO : @SemanticOmegaCofinalityLaws MF FI FO}
+  `{FDL : @SemanticMeasureDiagonalLaws MF FI FO}.
+
+Variable bind_cofinality : forall A R
+    (t : ptree E MN A) (k : A -> ptree E MN R),
+    operational_bind_cofinal (MF := MF) t k.
+
+Lemma stable_hitting_front_choice {A R} (k : A -> ptree E MN R) :
+  exists front : A -> MF (frontier_head E MN R),
+    forall a, stable_hitting_weak
+      (@ptree_primitive_kernel E MN MF FI MX R)
+      (observe (k a)) (front a).
+Proof.
+  assert (Hexists : forall a : A,
+      exists out : MF (frontier_head E MN R),
+        stable_hitting_weak
+          (@ptree_primitive_kernel E MN MF FI MX R)
+          (observe (k a)) out).
+  { intro a. apply stable_hitting_weak_exists. }
+  exact (choice
+    (fun a out => stable_hitting_weak
+      (@ptree_primitive_kernel E MN MF FI MX R)
+      (observe (k a)) out) Hexists).
+Qed.
+
+Lemma probabilistic_eutt_state_hitting_lift {R1 R2}
+    (RR : R1 -> R2 -> Prop)
+    (s1 : ptree' E MN R1) (s2 : ptree' E MN R2) out1 out2 :
+  probabilistic_eutt_state RR s1 s2 ->
+  stable_hitting_weak
+    (@ptree_primitive_kernel E MN MF FI MX R1) s1 out1 ->
+  stable_hitting_weak
+    (@ptree_primitive_kernel E MN MF FI MX R2) s2 out2 ->
+  sem_lift (ptree_stable_head_rel RR
+    (@probabilistic_eutt_state E MN MF FI FC MX FO R1 R2 RR)) out1 out2.
+Proof.
+  intros Hrel Hhit1 Hhit2.
+  apply stable_hitting_bisim_unfold in Hrel.
+  destruct Hrel as [Hforward _].
+  destruct (Hforward out1 Hhit1) as [out2' [Hhit2' Hlift]].
+  eapply sem_lift_proper_r; [|exact Hlift].
+  eapply stable_hitting_weak_unique; [exact Hhit2'|exact Hhit2].
+Qed.
+
+(** The coinduction candidate contains the already established greatest
+    fixed point as well as bind closure.  The first summand is the standard
+    coinduction-up-to-gfp device needed when a source return enters an
+    arbitrary related continuation. *)
+Definition bind_bisim_candidate (A : Type)
+    (s1 s2 : ptree' E MN A) : Prop :=
+  probabilistic_eutt_state eq s1 s2 \/
+  exists (R1 R2 : Type) (RR : R1 -> R2 -> Prop)
+    (t1 : ptree E MN R1) (t2 : ptree E MN R2)
+    (k1 : R1 -> ptree E MN A) (k2 : R2 -> ptree E MN A),
+    s1 = observe (PTree.bind t1 k1) /\
+    s2 = observe (PTree.bind t2 k2) /\
+    probabilistic_eutt RR t1 t2 /\
+    (forall r1 r2, RR r1 r2 -> probabilistic_eutt eq (k1 r1) (k2 r2)).
+
+Lemma bind_bisim_candidate_postfixed A :
+  forall s1 s2, bind_bisim_candidate (A := A) s1 s2 ->
+    stable_hitting_match
+      (@ptree_primitive_kernel E MN MF FI MX A)
+      (@ptree_primitive_kernel E MN MF FI MX A)
+      (@ptree_stable_head_rel E MN A A eq)
+      (bind_bisim_candidate (A := A)) s1 s2.
+Proof.
+  intros s1 s2 [Hknown|Hbind].
+  - apply stable_hitting_bisim_unfold in Hknown.
+    unfold stable_hitting_match in Hknown |- *.
+    destruct Hknown as [Hforward Hbackward]. split.
+    + intros out1 Hhit1. destruct (Hforward out1 Hhit1)
+        as [out2 [Hhit2 Hlift]]. exists out2. split; [exact Hhit2|].
+      eapply sem_lift_mono; [|exact Hlift].
+      apply ptree_stable_head_rel_mono.
+      intros x1 x2 Hrel. left. exact Hrel.
+    + intros out2 Hhit2. destruct (Hbackward out2 Hhit2)
+        as [out1 [Hhit1 Hlift]]. exists out1. split; [exact Hhit1|].
+      eapply sem_lift_mono; [|exact Hlift].
+      apply ptree_stable_head_rel_mono.
+      intros x1 x2 Hrel. left. exact Hrel.
+  - destruct Hbind as
+      [R1 [R2 [RR [t1 [t2 [k1 [k2 [-> [-> [Hsource Hk]]]]]]]]]].
+    apply probabilistic_eutt_unfold in Hsource.
+    unfold stable_hitting_match in Hsource |- *.
+    destruct Hsource as [Hforward Hbackward]. split.
+    + intros hs1 Hhit1.
+      destruct (stable_hitting_weak_exists
+        (@ptree_primitive_kernel E MN MF FI MX R1) (observe t1))
+        as [source1 Hsource1].
+      destruct (Hforward source1 Hsource1)
+        as [source2 [Hsource2 Hlift]].
+      destruct (stable_hitting_front_choice k1) as [front1 Hfront1].
+      destruct (stable_hitting_front_choice k2) as [front2 Hfront2].
+      assert (Hbound1 : stable_hitting_weak
+        (@ptree_primitive_kernel E MN MF FI MX A)
+        (observe (PTree.bind t1 k1))
+        (sem_bind source1 (frontier_head_bind_front k1 front1))).
+      { eapply stable_hitting_weak_bind;
+          [apply bind_cofinality|exact Hsource1|exact Hfront1]. }
+      assert (Hbound2 : stable_hitting_weak
+        (@ptree_primitive_kernel E MN MF FI MX A)
+        (observe (PTree.bind t2 k2))
+        (sem_bind source2 (frontier_head_bind_front k2 front2))).
+      { eapply stable_hitting_weak_bind;
+          [apply bind_cofinality|exact Hsource2|exact Hfront2]. }
+      exists (sem_bind source2 (frontier_head_bind_front k2 front2)). split.
+      * exact Hbound2.
+      * eapply sem_lift_proper_l.
+        -- eapply stable_hitting_weak_unique; [exact Hbound1|exact Hhit1].
+        -- eapply sem_lift_bind; [exact Hlift|].
+        intros h1 h2 Hhead. dependent destruction Hhead.
+        -- eapply sem_lift_mono.
+           ++ apply ptree_stable_head_rel_mono.
+              intros x1 x2 Hrel. left. exact Hrel.
+           ++ apply probabilistic_eutt_state_hitting_lift
+                with (s1 := observe (k1 r1)) (s2 := observe (k2 r2));
+                [exact (Hk r1 r2 H)|exact (Hfront1 r1)|exact (Hfront2 r2)].
+        -- apply sem_lift_ret. constructor. intro x. right.
+           exists R1, R2, RR, (k0 x), (k3 x), k1, k2.
+           repeat split; try reflexivity.
+           ++ exact (H x).
+           ++ exact Hk.
+    + intros hs2 Hhit2.
+      destruct (stable_hitting_weak_exists
+        (@ptree_primitive_kernel E MN MF FI MX R2) (observe t2))
+        as [source2 Hsource2].
+      destruct (Hbackward source2 Hsource2)
+        as [source1 [Hsource1 Hlift]].
+      destruct (stable_hitting_front_choice k1) as [front1 Hfront1].
+      destruct (stable_hitting_front_choice k2) as [front2 Hfront2].
+      assert (Hbound1 : stable_hitting_weak
+        (@ptree_primitive_kernel E MN MF FI MX A)
+        (observe (PTree.bind t1 k1))
+        (sem_bind source1 (frontier_head_bind_front k1 front1))).
+      { eapply stable_hitting_weak_bind;
+          [apply bind_cofinality|exact Hsource1|exact Hfront1]. }
+      assert (Hbound2 : stable_hitting_weak
+        (@ptree_primitive_kernel E MN MF FI MX A)
+        (observe (PTree.bind t2 k2))
+        (sem_bind source2 (frontier_head_bind_front k2 front2))).
+      { eapply stable_hitting_weak_bind;
+          [apply bind_cofinality|exact Hsource2|exact Hfront2]. }
+      exists (sem_bind source1 (frontier_head_bind_front k1 front1)). split.
+      * exact Hbound1.
+      * eapply sem_lift_proper_r.
+        -- eapply stable_hitting_weak_unique; [exact Hbound2|exact Hhit2].
+        -- eapply sem_lift_bind; [exact Hlift|].
+        intros h1 h2 Hhead. dependent destruction Hhead.
+        -- eapply sem_lift_mono.
+           ++ apply ptree_stable_head_rel_mono.
+              intros x1 x2 Hrel. left. exact Hrel.
+           ++ apply probabilistic_eutt_state_hitting_lift
+                with (s1 := observe (k1 r1)) (s2 := observe (k2 r2));
+                [exact (Hk r1 r2 H)|exact (Hfront1 r1)|exact (Hfront2 r2)].
+        -- apply sem_lift_ret. constructor. intro x. right.
+           exists R1, R2, RR, (k0 x), (k3 x), k1, k2.
+           repeat split; try reflexivity.
+           ++ exact (H x).
+           ++ exact Hk.
+Qed.
+
+(** Monadic congruence.  The only syntax-specific premise is the current
+    global form of the global/diagonal fuel cofinality theorem; it is used as
+    a proof-side scheduling fact by [stable_hitting_weak_bind], never by the
+    definition of [probabilistic_eutt]. *)
+Theorem probabilistic_eutt_bind : forall A R1 R2
+    (RR : R1 -> R2 -> Prop)
+    (t1 : ptree E MN R1) (t2 : ptree E MN R2)
+    (k1 : R1 -> ptree E MN A) (k2 : R2 -> ptree E MN A),
+  probabilistic_eutt RR t1 t2 ->
+  (forall r1 r2, RR r1 r2 -> probabilistic_eutt eq (k1 r1) (k2 r2)) ->
+  probabilistic_eutt eq (PTree.bind t1 k1) (PTree.bind t2 k2).
+Proof.
+  intros A R1 R2 RR t1 t2 k1 k2 Hsource Hk.
+  unfold probabilistic_eutt, probabilistic_eutt_state,
+    stable_hitting_bisim.
+  eapply (@leq_gfp _ _ (fstable_hitting_bisim
+    (@ptree_primitive_kernel E MN MF FI MX A)
+    (@ptree_primitive_kernel E MN MF FI MX A)
+    (@ptree_stable_head_rel_mono E MN A A eq))
+    (bind_bisim_candidate (A := A))).
+  - exact (bind_bisim_candidate_postfixed (A := A)).
+  - right. exists R1, R2, RR, t1, t2, k1, k2.
+    repeat split; try reflexivity; assumption.
+Qed.
+
+End ProbabilisticEuttBindCongruence.
